finish sn proof for one setup

OneSortHomArityGen/Progress.lean
@@ -1,8 +1,8 @@
 import LeanSubst
-import LeanSysF.Term
-import LeanSysF.Kinding
-import LeanSysF.Typing
-import LeanSysF.Reduction
+import OneSortHomArityGen.Term
+import OneSortHomArityGen.Kinding
+import OneSortHomArityGen.Typing
+import OneSortHomArityGen.Reduction
 
 open LeanSubst
 
@@ -16,19 +16,35 @@ def Term.is_tlam : Term -> Bool
 | .bind .tlam _ _ => true
 | _ => false
 
+@[simp]
+def ctor_neutral : Variant s n -> Vec Term n -> Bool
+| .app, ts => !(ts 0).is_lam
+| .tapp, ts => !(ts 0).is_tlam
+| _, _ => true
+
+theorem ctor_neutral_monotone (r : Ren)
+  : ctor_neutral v ts -> ctor_neutral v (λ i => (ts i)[r])
+:= by
+  intro h
+  cases v <;> simp at *
+  all_goals
+    generalize zdef : ts 0 = z at *
+    cases z <;> simp at *
+    case _ v _ _ =>
+    cases v <;> simp at *
+
 inductive Value : Term -> Prop where
 | var : Value #x
-| ctor {ts : Fin v.arity -> Term} :
-  ((h : v = .app) -> !(ts (by subst h; exact 0)).is_lam) ->
-  ((h : v = .tapp) -> !(ts (by subst h; exact 0)).is_tlam) ->
+| ctor {ts : Vec Term n} :
+  ctor_neutral v ts ->
   (∀ i, Value (ts i)) ->
   Value (.ctor v ts)
-| bind {ts : Fin v.arity -> Term} :
+| bind {ts : Vec Term n} :
   (∀ i, Value (ts i)) ->
   Value t ->
   Value (.bind v ts t)
 
-theorem Value.mk1 : Value t -> ∀ (a : Fin 1), Value (mk1 t a) := by
+theorem Value.mk1 : Value t -> ∀ (a : Fin 1), Value (v[t] a) := by
   intro v a
   cases a; case _ x p =>
   cases x; exact v
@@ -49,17 +65,31 @@ theorem Value.sound : Value t -> ∀ t', ¬ (t ~> t') := by
   intro h
   induction h
   case var => intro t' r; cases r
-  case ctor v ts j1 j2 j3 ih =>
+  case ctor n v ts j1 j2 ih =>
     intro t' r
     cases r
     case _ => simp at j1
-    case _ => simp at j2
+    case _ => simp at j1
     case _ i ts' h r => apply ih i _ r
   case bind t v ts j1 j2 ih1 ih2 =>
     intro t' r
     cases r
     case _ i ts' h r => apply ih1 i _ r
     case _ t' r => apply ih2 _ r
+
+theorem Value.monotone (r : Ren) : Value t -> Value t[r] := by
+  intro v; induction v generalizing r <;> simp
+  case var => apply Value.var
+  case ctor n v ts j1 j2 ih =>
+    apply Value.ctor
+    rw [ctor_neutral_monotone r j1]
+    intro i; apply ih i r
+  case bind n t v ts j1 j2 ih1 ih2 =>
+    apply Value.bind
+    intro i; apply ih1 i r
+    replace ih2 := ih2 r.lift
+    rw [Ren.to_lift (S := Term)] at ih2; simp at ih2
+    apply ih2
 
 theorem Kinding.value : Γ ⊢ A type -> Value A := by
   intro j; induction j
@@ -93,13 +123,13 @@ theorem progress t : Value t ∨ (∃ t', t ~> t') := by
               apply Or.inr
               generalize adef : ts 1 = a at *
               exists (t'[su a::+0])
-              rw [<-mk2_eta (t := ts)]
+              rw [<-Vec.eta2 (t := ts)]
               rw [zdef, adef]
-              rw [<-mk1_eta (t := ts')]
+              rw [<-Vec.eta1 (t := ts')]
               apply Red.beta
             all_goals solve | (
               apply Or.inl; apply Value.ctor
-              simp; rw [zdef]; simp
+              simp; rw [zdef]
               apply Value.mk2 ih1 ih2)
           all_goals solve | (
             rw [zdef] at ih1
@@ -133,19 +163,17 @@ theorem progress t : Value t ∨ (∃ t', t ~> t') := by
               apply Or.inr
               generalize adef : ts 1 = a at *
               exists (t'[su a::+0])
-              rw [<-mk2_eta (t := ts)]
+              rw [<-Vec.eta2 (t := ts)]
               rw [zdef, adef]; simp
               apply Red.tbeta
             all_goals solve | (
               apply Or.inl; apply Value.ctor
-              simp; simp; rw [zdef]
-              apply Value.mk2 ih1 ih2)
+              simp [*]; apply Value.mk2 ih1 ih2)
           all_goals solve | (
             rw [zdef] at ih1
             apply Or.inl
             apply Value.ctor
-            simp; simp; rw [zdef]
-            simp [*])
+            simp [*]; simp [*])
         case _ ih2 =>
           cases ih2; case _ t' ih2 =>
           apply Or.inr
@@ -193,7 +221,7 @@ theorem progress t : Value t ∨ (∃ t', t ~> t') := by
           cases ih2; case _ t' r =>
           apply Or.inr
           exists (:λ[ts 0] t'); simp
-          apply Red.bind2 r
+          apply Red.bind2 _ r
       case _ ih1 =>
         cases ih1; case _ t' r =>
         apply Or.inr
@@ -210,7 +238,7 @@ theorem progress t : Value t ∨ (∃ t', t ~> t') := by
         cases ih2; case _ t' r =>
         apply Or.inr
         exists (Λ t')
-        apply Red.bind2 r
+        apply Red.bind2 _ r
     case _ =>
       cases ih2
       case _ ih2 =>
@@ -221,4 +249,4 @@ theorem progress t : Value t ∨ (∃ t', t ~> t') := by
         cases ih2; case _ t' r =>
         apply Or.inr
         exists (:∀ t')
-        apply Red.bind2 r
+        apply Red.bind2 _ r
