LeanSysF/OneSortHomArityGen.lean
@@ -1,0 +1,13 @@
+
+import OneSortHomArityGen.FreeVar
+-- import OneSortHomArityGen.Infer
+import OneSortHomArityGen.Kinding
+import OneSortHomArityGen.Preservation
+import OneSortHomArityGen.Progress
+import OneSortHomArityGen.Reduction
+import OneSortHomArityGen.SN
+import OneSortHomArityGen.StrongNormalization
+import OneSortHomArityGen.Term
+import OneSortHomArityGen.Typing
+import OneSortHomArityGen.Utility
+import OneSortHomArityGen.Vec
