OneSortHomArityGen/Infer.lean
@@ -1,0 +1,212 @@
+import LeanSubst
+import OneSortHomArityGen.Typing
+
+open LeanSubst
+
+def Term.beq : Term -> Term -> Bool
+| var x, var y => x = y
+| ctor .star _, ctor .star _ => true
+| ctor .arr ts1, ctor .arr ts2 =>
+  Term.beq (ts1 0) (ts2 0) && Term.beq (ts1 1) (ts2 1)
+| ctor .app ts1, ctor .app ts2 =>
+  Term.beq (ts1 0) (ts2 0) && Term.beq (ts1 1) (ts2 1)
+| ctor .tapp ts1, ctor .tapp ts2 =>
+  Term.beq (ts1 0) (ts2 0) && Term.beq (ts1 1) (ts2 1)
+| bind .lam ts1 t1, bind .lam ts2 t2 =>
+  Term.beq (ts1 0) (ts2 0) && Term.beq t1 t2
+| bind .tlam _ t1, bind .tlam _ t2 => Term.beq t1 t2
+| bind .all _ t1, bind .all _ t2 => Term.beq t1 t2
+| _, _ => false
+
+instance : BEq Term where
+  beq := Term.beq
+
+instance : LawfulBEq Term where
+  rfl := by {
+    intro a; induction a
+    case var => simp [BEq.beq, Term.beq]
+    case bind v _ _ _ _ =>
+      cases v <;> simp [BEq.beq, Term.beq] at * <;> simp [*]
+    case ctor v _ _ =>
+      cases v <;> simp [BEq.beq, Term.beq] at * <;> simp [*]
+  }
+  eq_of_beq := by {
+    intro a b h
+    simp [BEq.beq] at h
+    fun_induction Term.beq <;> simp at *
+    case _ => exact h
+    case _ ih1 ih2 => rw [ih1 h.1, ih2 h.2]; simp
+    case _ ih1 ih2 => rw [ih1 h.1, ih2 h.2]; simp
+    case _ ih1 ih2 => rw [ih1 h.1, ih2 h.2]; simp
+    case _ ih1 ih2 => rw [ih1 h.1, ih2 h.2]; simp
+    case _ ih => rw [ih h]
+    case _ ih => rw [ih h]
+  }
+
+def Term.is_type (Γ : Ctx Term) : Term -> Bool
+| var x =>
+  match Γ[x] with
+  | ctor .star _ => true
+  | _ => false
+| ctor .arr ts => (ts 0).is_type Γ && (ts 1).is_type Γ
+| bind .all _ t => t.is_type (★::Γ)
+| _ => false
+
+theorem is_type_sound : A.is_type Γ -> Γ ⊢ A type := by
+  intro h; fun_induction Term.is_type
+  case _ t ih =>
+    apply Kinding.var; simp at *
+    apply ih
+  case _ h => cases h
+  case _ ts ih1 ih2 =>
+    simp at h; rcases h with ⟨h1, h2⟩
+    rw [<-Vec.eta2 ts]; apply Kinding.arr
+    apply ih1 h1; apply ih2 h2
+  case _ ts t ih =>
+    simp; apply Kinding.all
+    apply ih h
+  case _ => cases h
+
+def Term.is_all : Term -> Option Term
+| bind .all _ t => t
+| _ => none
+
+def Term.is_arr : Term -> Option (Term × Term)
+| ctor .arr ts => (ts 0, ts 1)
+| _ => none
+
+def Term.pred (ℓ : Nat) : Term -> Option Term
+| var x => if x > ℓ then var (x - 1) else none
+| ctor .star ts => ctor .star ts
+| ctor .arr ts => do
+  let A <- Term.pred ℓ (ts 0)
+  let B <- Term.pred ℓ (ts 1)
+  ctor .arr v[A, B]
+| ctor .app ts => do
+  let A <- Term.pred ℓ (ts 0)
+  let B <- Term.pred ℓ (ts 1)
+  ctor .arr v[A, B]
+| ctor .tapp ts => do
+  let A <- Term.pred ℓ (ts 0)
+  let B <- Term.pred ℓ (ts 1)
+  ctor .arr v[A, B]
+| bind .all ts t => do
+  let P <- Term.pred (ℓ + 1) t
+  bind .all ts P
+| bind .lam ts t => do
+  let A <- Term.pred ℓ (ts 0)
+  let b <- Term.pred (ℓ + 1) t
+  bind .lam v[A] b
+| bind .tlam ts t => do
+  let b <- Term.pred (ℓ + 1) t
+  bind .all ts b
+
+def infer (Γ : Ctx Term) : Term -> Option Term
+| .var x =>
+  let A := Γ[x]
+  if A.is_type Γ then A else none
+| .ctor .app ts => do
+  let f := ts 0
+  let a := ts 1
+  let F <- infer Γ f
+  let A' <- infer Γ a
+  let (A, B) <- F.is_arr
+  if A' == A then B
+  else none
+| .ctor .tapp ts => do
+  let f := ts 0
+  let a := ts 1
+  let F <- infer Γ f
+  let P <- F.is_all
+  if a.is_type Γ then P[su a::+0]
+  else none
+| .bind .lam ts t => do
+  let A := ts 0
+  let B <- infer (A::Γ) t
+  let B <- Term.pred 0 B
+  if A.is_type Γ then A -:> B
+  else none
+| .bind .tlam ts t => do
+  let P <- infer (★::Γ) t
+  :∀ P
+| _ => none
+
+-- TODO: too lazy to prove this right now
+-- How to do it: generalize to ℓ and an iterated lift of +1 by ℓ (similar to free vars stuff)
+-- That gives you a strong enough inductive hypothesis to prove this for all ℓ
+-- then the 0 case is an easy corollary
+--
+-- Might be bugs in Term.pred itself, but clearly it is a definable function
+theorem Term.pred_sound : Term.pred 0 t = some p -> t = p[+1] := by
+  sorry
+
+theorem Term.is_all_some : Term.is_all t = some P -> t = :∀ P := by
+  intro h
+  cases t <;> simp [Term.is_all] at h
+  case _ n v ts t =>
+  cases v <;> simp at h; subst h; simp
+
+theorem Term.is_arr_some : Term.is_arr t = some F -> ∃ A B, t = A -:> B ∧ F = (A, B) := by
+  intro h
+  cases t <;> simp [Term.is_arr] at h
+  case _ n v ts =>
+  cases v <;> simp at h; subst h
+  exists ts 0; exists ts 1; simp
+
+theorem infer_sound : infer Γ t = some A -> Γ ⊢ t : A := by
+  intro h; fun_induction infer generalizing A
+  case _ Γ x A' h2 =>
+    subst A'; injection h with e; subst e
+    apply Typing.var rfl
+    apply is_type_sound h2
+  case _ => cases h
+  case _ Γ ts f a ih1 ih2 =>
+    replace h := Option.bind_eq_some_iff.1 h
+    rcases h with ⟨u1, h1, h2⟩
+    replace h2 := Option.bind_eq_some_iff.1 h2
+    rcases h2 with ⟨u2, h2, h3⟩
+    replace h3 := Option.bind_eq_some_iff.1 h3
+    rcases h3 with ⟨u3, h3, h4⟩
+    simp at h4; rcases h4 with ⟨h4, h5⟩
+    replace h3 := Term.is_arr_some h3
+    rcases h3 with ⟨A', B, h3, h6⟩
+    subst h4 h3 h6; simp at h5; subst h5
+    rw [<-Vec.eta2 ts]; apply Typing.app
+    apply ih1 h1
+    apply ih2 h2
+  case _ Γ ts f a ih =>
+    replace h := Option.bind_eq_some_iff.1 h
+    rcases h with ⟨u1, h1, h2⟩
+    replace h2 := Option.bind_eq_some_iff.1 h2
+    rcases h2 with ⟨u2, h2, h3⟩; simp at h3
+    rcases h3 with ⟨h3, h4⟩
+    replace h2 := Term.is_all_some h2; subst h2 h4
+    rw [<-Vec.eta2 ts]; apply Typing.tapp
+    apply ih h1
+    apply is_type_sound h3
+    simp [a]
+  case _ Γ ts t A' ih =>
+    simp at h
+    replace h := Option.bind_eq_some_iff.1 h
+    rcases h with ⟨u1, h1, h2⟩
+    replace h2 := Option.bind_eq_some_iff.1 h2
+    rcases h2 with ⟨u2, h2, h4⟩
+    replace h2 := Term.pred_sound h2
+    simp at h4; rcases h4 with ⟨h4, h5⟩; subst h2 h5
+    rw [<-Vec.eta1 ts]; apply Typing.lam
+    apply is_type_sound h4
+    apply ih h1
+  case _ Γ ts t ih =>
+    replace h := Option.bind_eq_some_iff.1 h
+    rcases h with ⟨u1, h1, h2⟩; simp
+    injection h2 with e; subst e
+    apply Typing.tlam
+    apply ih h1
+  case _ => cases h
+
+def ex0 : Term := :∀ #0 -:> #0
+def ex1 : Term := Λ :λ[#0] #0
+def ex2 : Term := ex1 :@[ex0] :@ ex1
+
+#eval infer Ctx.nil ex1
+#eval infer Ctx.nil ex2
