OneSortHomArityGen/Reduction.lean
@@ -1,0 +1,601 @@
+
+import LeanSubst
+import LeanSubst.Reduction
+import OneSortHomArityGen.Term
+
+open LeanSubst
+
+inductive Red : Term -> Term -> Prop where
+| beta {A b t : Term} : Red ((:λ[A] b) :@ t) (b[su t::+0])
+| tbeta {b t : Term} : Red ((Λ b) :@[t]) (b[su t::+0])
+| ctor v i {ts ts'} :
+  (∀ j ≠ i, ts j = ts' j) ->
+  Red (ts i) (ts' i) ->
+  Red (.ctor v ts) (.ctor v ts')
+| bind1 v i {ts ts' t} :
+  (∀ j ≠ i, ts j = ts' j) ->
+  Red (ts i) (ts' i) ->
+  Red (.bind v ts t) (.bind v ts' t)
+| bind2 v {ts t t'} :
+  Red t t' ->
+  Red (.bind v ts t) (.bind v ts t')
+
+infix:80 " ~> " => Red
+infix:81 " ~>* " => Star Red
+infix:80 " ~>a " => ActionRed Red
+
+@[app_unexpander Star]
+def unexpandStar_Red : Lean.PrettyPrinter.Unexpander
+| `($_ Red $s $t) => `($s ~>* $t)
+| _ => throw ()
+
+@[app_unexpander ActionRed]
+def unexpandActionRed_Red : Lean.PrettyPrinter.Unexpander
+| `($_ Red $s $t) => `($s ~>a $t)
+| _ => throw ()
+
+theorem Red.antirename {s t : Term} (r : Ren) :
+  s[r] ~> t ->
+  ∃ z, s ~> z ∧ t = z[r]
+:= by
+  intro h
+  generalize wdef : s[r:Term] = w at *
+  induction h generalizing s r
+  case beta A b t =>
+    cases s <;> simp at wdef
+    case ctor n v ts =>
+    rcases wdef with ⟨e1, e2, e3⟩
+    subst e1; subst e2; simp at *
+    rcases e3 with ⟨e3, e4⟩; subst e4
+    generalize wdef : ts 0 = w at *
+    cases w <;> simp at e3
+    case _ n v ts' t =>
+    rcases e3 with ⟨e3, e4, e5, e6⟩
+    subst e3; subst e4; simp at *
+    subst e5; subst e6; simp
+    exists (t[su (ts 1)::+0]); apply And.intro
+    rw [<-Vec.eta2 ts, wdef]; simp
+    rw [<-Vec.eta1 ts']; apply Red.beta
+    simp
+  case tbeta b t =>
+    cases s <;> simp at wdef
+    case ctor n v ts =>
+    rcases wdef with ⟨e1, e2, e3⟩
+    subst e1; subst e2; simp at e3
+    rcases e3 with ⟨e3, e4⟩; subst e4
+    generalize wdef : ts 0 = w at *
+    cases w <;> simp at e3
+    case _ n v ts' t =>
+    rcases e3 with ⟨e3, e4, e5, e6⟩
+    subst e3; subst e4; simp at *
+    subst e6; simp
+    exists (t[su (ts 1)::+0]); apply And.intro
+    rw [<-Vec.eta2 ts, wdef]; simp; apply Red.tbeta
+    simp
+  case ctor x v i ts ts' j1 j2 ih =>
+    cases s <;> simp at wdef
+    case _ n v' ts'' =>
+    rcases wdef with ⟨e1, e2, e3⟩; subst e1; simp at *
+    subst e2; subst e3; simp at *
+    replace ih := @ih (ts'' i) r rfl
+    rcases ih with ⟨z, h1, h2⟩
+    exists (.ctor v' (Vec.update i z ts'')); simp
+    apply And.intro
+    apply Red.ctor v' i
+    apply Vec.update_stable; simp
+    simp; apply h1
+    funext; case _ j =>
+    cases decEq j i
+    case _ h3 => rw [Vec.update_neq j h3]; simp [*]
+    case _ h3 => subst h3; simp [*]
+  case bind1 x v i ts ts' t j1 j2 ih =>
+    cases s <;> simp at wdef
+    case _ n v' ts'' t' =>
+    rcases wdef with ⟨e1, e2, e3, e4⟩
+    subst e1; subst e2; simp at *; subst e3; subst e4
+    replace ih := @ih (ts'' i) r rfl
+    rcases ih with ⟨z, h1, h2⟩
+    exists (.bind v' (Vec.update i z ts'') t'); simp
+    apply And.intro
+    apply Red.bind1 v' i
+    apply Vec.update_stable; simp
+    simp; apply h1
+    funext; case _ j =>
+    cases decEq j i
+    case _ h3 => rw [Vec.update_neq j h3]; simp [*]
+    case _ h3 => subst h3; simp [*]
+  case bind2 x v ts t t' j ih =>
+    cases s <;> simp at wdef
+    case _ i v' ts' t'' =>
+    rcases wdef with ⟨e1, e2, e3, e4⟩
+    subst e1; subst e2; simp at e3; subst e3; subst e4
+    replace ih := @ih t'' (r.lift)
+    rw [Ren.to_lift (S := Term)] at ih; simp at ih
+    rcases ih with ⟨z, h1, h2⟩
+    exists (Term.bind v' ts' z); apply And.intro
+    apply Red.bind2 _ h1; subst h2; simp
+    rw [Ren.to_lift (S := Term)]; simp
+
+theorem Red.ctor_star_lemma {ts ts'} i :
+  (∀ j ≠ i, ts j = ts' j) ->
+  ts i ~>* ts' i ->
+  .ctor v ts ~>* .ctor v ts'
+:= by
+  intro h1 r
+  generalize sdef : ts i = s at *
+  generalize tdef : ts' i = t at *
+  induction r generalizing ts ts' i
+  case _ =>
+    have lem : ts = ts' := by
+      funext; case _ x =>
+      cases decEq x i with
+      | isFalse h3 => apply h1 _ h3
+      | isTrue h3 => rw [h3, sdef, tdef]
+    rw [lem]; apply Star.refl
+  case _ y z r1 r2 ih =>
+    subst sdef; subst tdef
+    replace ih := @ih ts (Vec.update i y ts') i (Vec.update_stable _ _ h1) rfl Vec.update_eq
+    apply Star.step ih
+    apply Red.ctor v i Vec.update_neq; simp; exact r2
+
+theorem Red.ctor_star {ts ts' : Vec Term n}:
+  (∀ i, ts i ~>* ts' i) ->
+  .ctor v ts ~>* .ctor v ts'
+:= by
+  intro h
+  cases v <;> simp at *
+  case star => apply Star.refl
+  all_goals
+    rw [<-Vec.eta2 ts, <-Vec.eta2 ts']
+    apply Star.trans
+    apply Red.ctor_star_lemma (ts' := v[ts' 0, ts 1]) 0 _ _
+    simp; apply h.1; simp
+    apply Red.ctor_star_lemma 1 _ _
+    simp; apply h.2
+
+theorem Red.bind1_star_lemma {ts ts'} i :
+  (∀ j ≠ i, ts j = ts' j) ->
+  ts i ~>* ts' i ->
+  .bind v ts t ~>* .bind v ts' t
+:= by
+  intro h r
+  generalize udef : ts i = u at *
+  generalize wdef : ts' i = w at *
+  induction r generalizing ts ts' i
+  case _ =>
+    have lem : ts = ts' := by
+      funext; case _ x =>
+      cases decEq x i with
+      | isFalse h3 => apply h _ h3
+      | isTrue h3 => rw [h3, udef, wdef]
+    rw [lem]; apply Star.refl
+  case _ v y z r1 r2 ih =>
+    subst udef; subst wdef
+    replace ih := @ih ts (Vec.update i y ts') i (Vec.update_stable _ _ h) rfl Vec.update_eq
+    apply Star.step ih
+    apply Red.bind1 v i Vec.update_neq; simp; exact r2
+
+theorem Red.bind2_star_lemma {t t'} :
+  t ~>* t' ->
+  .bind v ts t ~>* .bind v ts t'
+:= by
+  intro r
+  induction r
+  case _ => apply Star.refl
+  case _ y z r1 r2 ih =>
+    apply Star.step ih
+    apply Red.bind2 _ r2
+
+theorem Red.bind_star {ts ts' : Vec Term n}:
+  (∀ i, ts i ~>* ts' i) ->
+  t ~>* t' ->
+  .bind v ts t ~>* .bind v ts' t'
+:= by
+  intro r1 r2
+  cases v <;> simp at *
+  case lam =>
+    rw [<-Vec.eta1 ts, <-Vec.eta1 ts']
+    apply Star.trans; apply Red.bind2_star_lemma r2
+    apply Red.bind1_star_lemma 0; simp; simp; apply r1
+  all_goals apply Red.bind2_star_lemma r2
+
+theorem Red.subst {t t'} (σ : Subst Term) :
+  t ~> t' ->
+  t[σ] ~> t'[σ]
+:= by
+  intro h
+  induction h generalizing σ
+  case beta A b t =>
+    simp; have lem := @Red.beta A[σ] (b[.re 0 :: σ ∘ +1]) (t[σ])
+    simp at lem; apply lem
+  case tbeta b t =>
+    simp; have lem := @Red.tbeta (b[.re 0 :: σ ∘ +1]) (t[σ])
+    simp at lem; apply lem
+  case ctor v i ts ts' h r ih =>
+    simp; apply Red.ctor _ i
+    intro j e; rw [h j e]
+    apply ih σ
+  case bind1 v i ts ts' t h1 h2 ih =>
+    simp; apply Red.bind1 _ i
+    intro j e; rw [h1 j e]
+    apply ih σ
+  case bind2 r ih =>
+    simp; apply Red.bind2
+    replace ih := ih σ.lift; simp at ih
+    apply ih
+
+theorem Red.subst_action_lift {σ τ : Subst Term} :
+  (∀ i, σ i ~>a τ i) ->
+  ∀ i, σ.lift i ~>a τ.lift i
+:= by
+  intro h i
+  cases i <;> simp
+  apply ActionRed.re
+  case _ x =>
+  simp [Subst.compose]
+  replace h := h x
+  generalize udef : σ x = u at *
+  generalize vdef : τ x = v at *
+  cases h <;> simp
+  case _ r => apply ActionRed.su; apply Red.subst _ r
+  case _ => apply ActionRed.re
+
+theorem Red.subst_action (σ τ : Subst Term) :
+  (∀ i, σ i ~>a τ i) ->
+  t[σ] ~>* t[τ]
+:= by
+  intro h
+  induction t generalizing σ τ <;> simp
+  case var x =>
+    replace h := h x
+    generalize adef : σ x = a at *
+    generalize bdef : τ x = b at *
+    cases h <;> simp
+    case _ r => apply Star.step Star.refl r
+    case _ => apply Star.refl
+  case ctor v ts ih =>
+    apply Red.ctor_star
+    intro i; apply ih i _ _ h
+  case bind v ts' t ih1 ih2 =>
+    apply Red.bind_star
+    intro i; apply ih1 i _ _ h
+    replace ih2 := ih2 σ.lift τ.lift (Red.subst_action_lift h)
+    simp at ih2; apply ih2
+
+theorem Red.app1 : f ~> f' -> (f :@ a) ~> (f' :@ a) := by
+  intro r; apply Red.ctor .app 0 _
+  apply r
+  intro j h
+  cases j; case _ v p =>
+  cases v <;> simp at *
+  case _ j =>
+  cases j; simp
+  omega
+
+theorem Red.app_inv :
+  (f:@ a) ~> t ->
+    (∃ A b, (f = :λ[A] b) ∧ t = b[su a::+0])
+    ∨ (∃ f', t = f':@ a ∧ f ~> f')
+    ∨ (∃ a', t = f :@ a' ∧ a ~> a')
+:= by
+  intro r; generalize zdef : (f:@ a) = z at r
+  cases r <;> simp at zdef
+  case beta A b t =>
+    cases zdef; case _ e1 e2 =>
+    subst e1; subst e2
+    apply Or.inl; simp
+    exists A; exists b
+  case ctor v i ts ts' r1 r2 =>
+    rcases zdef with ⟨e1, e2, e3⟩
+    subst e1; subst e2; simp at e3
+    rcases e3 with ⟨e3, e4⟩; subst e3; subst e4
+    cases i using Fin.cases2
+    case _ =>
+      apply Or.inr; apply Or.inl
+      exists (ts' 0); simp [*]
+    case _ =>
+      apply Or.inr; apply Or.inr
+      exists (ts' 1); simp [*]
+
+theorem Red.tapp1 : f ~> f' -> (f :@[a]) ~> (f' :@[a]) := by
+  intro r; apply Red.ctor .tapp 0 _
+  apply r; intro j h
+  cases j using Fin.cases2
+  case _ => exfalso; apply h rfl
+  case _ => simp
+
+theorem Red.tapp_inv :
+  (f:@[a]) ~> t ->
+    (∃ b, (f = Λ b) ∧ t = b[su a::+0])
+    ∨ (∃ f', t = f':@[a] ∧ f ~> f')
+    ∨ (∃ a', t = f :@[a'] ∧ a ~> a')
+:= by
+  intro r; generalize zdef : (f:@[a]) = z at r
+  cases r <;> simp at zdef
+  case tbeta b t =>
+    rcases zdef with ⟨e1, e2⟩
+    subst e1 e2; apply Or.inl
+    exists b
+  case ctor n v i ts ts' h r =>
+    rcases zdef with ⟨e1, e2, e3⟩
+    subst e1 e2 e3
+    cases i using Fin.cases2 <;> simp at *
+    apply Or.inr; apply Or.inl
+    subst h; exists ts' 0
+    apply Or.inr; apply Or.inr
+    subst h; exists ts' 1
+
+theorem Red.lam_inv :
+  (:λ[A] b) ~> t ->
+    (∃ A', (t = :λ[A'] b) ∧ A ~> A')
+    ∨ (∃ b', (t = :λ[A] b') ∧ b ~> b')
+:= by
+  intro r; generalize zdef : (:λ[A] b) = z at r
+  cases r <;> simp at zdef
+  case bind1 n v i ts ts' t h r =>
+    rcases zdef with ⟨e1, e2, e3, e4⟩
+    subst e1 e2 e3 e4
+    cases i using Fin.cases1; simp at *
+    apply Or.inl r
+  case bind2 n v ts t t' r =>
+    rcases zdef with ⟨e1, e2, e3, e4⟩
+    subst e1 e2 e3 e4
+    apply Or.inr; exists t'
+
+theorem Red.tlam_inv : (Λ b) ~> t -> (∃ b', (t = Λ b') ∧ b ~> b') := by
+  intro r; generalize zdef : (Λ b) = z at r
+  cases r <;> simp at zdef
+  case bind1 n v i ts ts' t h r =>
+    rcases zdef with ⟨e1, e2, e3, e4⟩
+    subst e1 e2 e3 e4
+    apply Fin.elim0 i
+  case bind2 n v ts t t' r =>
+    rcases zdef with ⟨e1, e2, e3, e4⟩
+    subst e1 e2 e3 e4; exists t'
+
+instance : Substitutive Red where
+  subst := Red.subst
+
+-- inductive ParRed : Term -> Term -> Prop where
+-- | star : ParRed ★ ★
+-- | var {x} : ParRed (#x) (#x)
+-- | arr {A B} : ParRed (A -:> B) (A -:> B)
+-- | all {P} : ParRed (:∀ P) (:∀ P)
+-- | beta {A b b' t t'} :
+--   ParRed b b' ->
+--   ParRed t t' ->
+--   ParRed ((:λ[A] b) :@ t) (b'[.su t'::I])
+-- | app {f f' a a'} :
+--   ParRed f f' ->
+--   ParRed a a' ->
+--   ParRed (f :@ a) (f' :@ a')
+-- | lam {A A' t t'} :
+--   ParRed A A' ->
+--   ParRed t t' ->
+--   ParRed (:λ[A] t) (:λ[A'] t')
+
+-- infix:80 " ~p> " => ParRed
+-- infix:81 " ~p>* " => Star ParRed
+
+-- inductive ParRedSubstAction : Subst.Action Term -> Subst.Action Term -> Prop where
+-- | su {t t'} : t ~p> t' -> ParRedSubstAction (.su t) (.su t')
+-- | re {x} : ParRedSubstAction (.re x) (.re x)
+
+-- infix:80 " ~ps> " => ParRedSubstAction
+-- infix:81 " ~ps>* " => Star ParRedSubstAction
+
+-- namespace ParRed
+--   theorem refl {t} : t ~p> t := by
+--     induction t
+--     case star => apply ParRed.star
+--     case arr => apply ParRed.arr
+--     case all => apply ParRed.all
+--     case var => apply ParRed.var
+--     case app ih1 ih2 => apply ParRed.app ih1 ih2
+--     case lam ih => apply ParRed.lam ih
+
+--   @[simp]
+--   def complete : Term -> Term
+--   | .app (.lam _ b) t =>
+--     let b' := complete b
+--     let t' := complete t
+--     b'[.su t'::I]
+--   | .app f a =>
+--     let f' := complete f
+--     let a' := complete a
+--     .app f' a'
+--   | .lam A t => .lam A (complete t)
+--   | .var k x => .var k x
+--   | .star => .star
+--   | .arr A B => .arr A B
+--   | .all P => .all P
+
+--   theorem subst {t t'} (σ : Subst Term) :
+--     t ~p> t' ->
+--     t[σ] ~p> t'[σ]
+--   := by
+--     intro h
+--     induction h generalizing σ
+--     case star => sorry
+--     case arr => sorry
+--     case all => sorry
+--     case var => apply ParRed.refl
+--     case beta A b b' t t' r1 r2 ih1 ih2 =>
+--       simp; have lem1 := @ParRed.beta A
+--         (b[.re 0 :: σ ∘ S]) (b'[.re 0 :: σ ∘ S])
+--         (t[σ]) (t'[σ])
+--       simp at lem1; apply lem1
+--       apply ih1; apply ih2
+--     case app r1 r2 ih1 ih2 =>
+--       simp; apply ParRed.app
+--       apply ih1; apply ih2
+--     case lam r ih =>
+--       simp; apply ParRed.lam; apply ih
+
+--   theorem subst_action {x} {σ σ' : Subst Term} (r : Ren) :
+--     σ x ~ps> σ' x ->
+--     (σ ∘ r.to) x ~ps> (σ' ∘ r.to) x
+--   := by
+--     intro h
+--     unfold Subst.compose; simp
+--     generalize zdef : σ x = z at *
+--     generalize zpdef : σ' x = z' at *
+--     cases z <;> cases z'
+--     all_goals (cases h; try simp [*])
+--     apply ParRedSubstAction.re
+--     case _ r =>
+--       apply ParRedSubstAction.su
+--       apply subst _ r
+
+--   theorem subst_red_lift {σ σ' : Subst Term} :
+--     (∀ x, σ x ~ps> σ' x) ->
+--     ∀ x, σ.lift x ~ps> σ'.lift x
+--   := by
+--     intro h x
+--     cases x <;> simp
+--     case _ => apply ParRedSubstAction.re
+--     case _ x =>
+--       have lem := subst_action (· + 1) (h x); simp at lem
+--       apply lem
+
+--   theorem hsubst {t t'} {σ σ' : Subst Term} :
+--     (∀ x, σ x ~ps> σ' x) ->
+--     t ~p> t' ->
+--     t[σ] ~p> t'[σ']
+--   := by
+--     intro h1 h2; induction t generalizing t' σ σ'
+--     case star => sorry
+--     case arr => sorry
+--     case all => sorry
+--     case var x =>
+--       cases h2; simp
+--       replace h1 := h1 x
+--       generalize zdef : σ x = z at *
+--       generalize zpdef : σ' x = z' at *
+--       cases z <;> cases z'
+--       all_goals (cases h1; try simp [*])
+--       apply refl
+--     case app f a ih1 ih2 =>
+--       cases h2 <;> simp at *
+--       case beta A b b' t r1 r2 =>
+--         have lem1 := @ParRed.beta A (b[.re 0 :: σ ∘ S]) (b'[.re 0 :: σ' ∘ S]) (a[σ]) (t[σ'])
+--         simp at lem1; apply lem1 _
+--         apply ih2 h1 r2
+--         have lem2 := ih1 h1 (ParRed.lam r1); simp at lem2
+--         cases lem2; case _ lem2 =>
+--         apply lem2
+--       case app f' a' r1 r2 =>
+--         apply ParRed.app
+--         apply ih1 h1 r1
+--         apply ih2 h1 r2
+--     case lam t ih =>
+--       cases h2; case _ t' h2 =>
+--       simp; apply ParRed.lam
+--       have lem := @ih t' σ.lift σ'.lift (subst_red_lift h1) h2
+--       simp at lem; apply lem
+
+--   theorem triangle {t s} : t ~p> s -> s ~p> complete t := by
+--     intro r; induction r <;> simp at *
+--     case star => sorry
+--     case arr => sorry
+--     case all => sorry
+--     case var => apply ParRed.refl
+--     case beta ih1 ih2 =>
+--       apply hsubst
+--       intro x; cases x <;> simp
+--       apply ParRedSubstAction.su; apply ih2
+--       apply ParRedSubstAction.re; apply ih1
+--     case app f f' a a' r1 r2 ih1 ih2 =>
+--       cases f <;> simp at *
+--       case star => sorry
+--       case arr => sorry
+--       case all => sorry
+--       case var => apply ParRed.app ih1 ih2
+--       case app => apply ParRed.app ih1 ih2
+--       case lam =>
+--         cases r1; case _ r1 =>
+--         cases ih1; case _ ih1 =>
+--         apply ParRed.beta ih1 ih2
+--     case lam ih => apply ParRed.lam ih
+
+--   instance : Substitutive ParRed where
+--     subst := subst
+
+--   instance : HasTriangle ParRed where
+--     complete := complete
+--     triangle := triangle
+-- end ParRed
+
+-- namespace Red
+--   theorem subst {t t'} (σ : Subst Term) :
+--     t ~> t' ->
+--     t[σ] ~> t'[σ]
+--   := by
+--     intro h
+--     induction h generalizing σ
+--     case beta A b t =>
+--       simp; have lem1 := @Red.beta A (b[.re 0 :: σ ∘ S]) (t[σ])
+--       simp at lem1; apply lem1
+--     case app1 ih =>
+--       simp; apply Red.app1 (ih σ)
+--     case app2 ih =>
+--       simp; apply Red.app2 (ih σ)
+--     case lam ih =>
+--       simp; apply Red.lam
+--       apply ih
+
+--   theorem seq_implies_par {t t'} : t ~> t' -> t ~p> t' := by
+--     intro h; induction h
+--     case beta => apply ParRed.beta ParRed.refl ParRed.refl
+--     case app1 r ih => apply ParRed.app ih ParRed.refl
+--     case app2 r ih => apply ParRed.app ParRed.refl ih
+--     case lam r ih => apply ParRed.lam ih
+
+--   theorem seqs_implies_pars {t t'} : t ~>* t' -> t ~p>* t' := by
+--     intro h; induction h
+--     case _ => apply Star.refl
+--     case _ y z r1 r2 ih =>
+--       replace r2 := seq_implies_par r2
+--       apply Star.step ih r2
+
+--   theorem par_implies_seqs {t t'} : t ~p> t' -> t ~>* t' := by
+--     intro h; induction h
+--     case star => sorry
+--     case arr => sorry
+--     case all => sorry
+--     case var => apply Star.refl
+--     case beta A b b' q q' r1 r2 ih1 ih2 =>
+--       have lem : (:λ[A] b) ~>* (:λ[A] b') := by
+--         apply Star.congr1 (Term.lam A) (@Red.lam A) ih1
+--       apply Star.trans
+--       apply Star.congr2 Term.app Red.app1 Red.app2 lem ih2
+--       apply Star.step Star.refl
+--       apply Red.beta
+--     case app f f' a a' r1 r2 ih1 ih2 =>
+--       apply Star.congr2 Term.app Red.app1 Red.app2 ih1 ih2
+--     case lam t t' A r ih =>
+--       apply Star.congr1 (Term.lam A) (@Red.lam A) ih
+
+--   theorem pars_implies_seqs {t t'} : t ~p>* t' -> t ~>* t' := by
+--     intro h; induction h
+--     case _ => apply Star.refl
+--     case _ y z r1 r2 ih =>
+--       replace r2 := par_implies_seqs r2
+--       apply Star.trans ih r2
+
+--   theorem confluence {s t1 t2} : s ~>* t1 -> s ~>* t2 -> ∃ t, t1 ~>* t ∧ t2 ~>* t := by
+--     intro h1 h2
+--     have lem1 := seqs_implies_pars h1
+--     have lem2 := seqs_implies_pars h2
+--     have lem3 := HasConfluence.confluence lem1 lem2
+--     cases lem3; case _ w lem3 =>
+--     have lem4 := pars_implies_seqs lem3.1
+--     have lem5 := pars_implies_seqs lem3.2
+--     exists w
+
+--   instance : Substitutive Red where
+--     subst := subst
+
+--   instance : HasConfluence Red where
+--     confluence := confluence
+-- end Red
