OneSortHomArityGen/SN.lean
@@ -1,0 +1,16 @@
+import LeanSubst
+import OneSortHomArityGen.Term
+import OneSortHomArityGen.Reduction
+import OneSortHomArityGen.Progress
+
+open LeanSubst
+
+theorem SN.var : SN Red #0 := by
+  apply SN.sn; intro y r; cases r
+
+theorem SN.monotone {t : Term} (r : Ren) : SN Red t -> SN Red t[r] := by
+  intro h; induction h generalizing r; case _ t h ih =>
+  apply SN.sn; intro y h2
+  replace h2 := Red.antirename r h2
+  rcases h2 with ⟨z, h2, h3⟩; subst h3
+  apply ih _ h2
