OneSortHomArityGen/StrongNormalization.lean
@@ -1,0 +1,565 @@
+
+import LeanSubst
+import OneSortHomArityGen.Term
+import OneSortHomArityGen.Kinding
+import OneSortHomArityGen.Typing
+import OneSortHomArityGen.Reduction
+import OneSortHomArityGen.Progress
+import OneSortHomArityGen.SN
+
+open LeanSubst
+
+-- Heavily following Lectures in Curry-Howard and the autosubst work:
+--
+-- Lectures on the Curry-Howard Isomorphism
+-- https://github.com/rocq-community/autosubst/blob/master/examples/ssr/SystemF_SN.v
+
+-- Notable differences:
+-- 1. Syntax/substitutions are single-sorted
+-- -- The Rocq development uses multisorted syntax/substitutions
+-- 2. Reduction is full (in particular we have all congruences rules)
+-- -- The Rocq development does not have congruence rules for type-positions
+-- 3. [2] forces a restriction on type instantiation; we choose Value
+-- 4. [3] forces us to know that A[σ] value when Γ ⊢ A type, which in turn requires that the
+--    logial relation is Kripke
+-- 5. [4] also requires a 4th property of candidates (monotonicity of renaming)
+
+-- Shallow neutral, turns out to be enough
+@[simp]
+def Term.not_lam : Term -> Bool
+| bind .lam _ _ => false
+| bind .tlam _ _ => false
+| _ => true
+
+namespace Normalization.Verison1
+
+-- Setup for semantic typing
+@[simp]
+abbrev Cand := Term -> Prop
+
+structure Reducible (P : Cand) : Prop where
+  subset : ∀ {t}, P t -> SN Red t
+  closed : ∀ {s t}, P s -> s ~> t -> P t
+  neu_acc : ∀ {s}, s.not_lam -> (∀ t, s ~> t -> P t) -> P s
+  mono : ∀ {t} (r : Ren), P t -> P t[r]
+
+def Admissible : (Nat -> Cand) -> Prop
+| ξ => ∀ x, Reducible (ξ x)
+
+@[simp]
+def LR (ξ : Nat -> Cand) : Term -> Cand
+| #x => ξ x
+| .ctor .arr ts => λ t => ∀ (r:Ren) a, LR ξ (ts 0) a -> LR ξ (ts 1) (t[r] :@ a)
+| .bind .all _ P => λ t => ∀ (r:Ren) C a, Reducible C -> Value a -> LR (C::ξ) P (t[r] :@[a])
+| _ => λ t => SN Red t
+
+def ΓR (ξ : Nat -> Cand) : Ctx Term -> (Subst Term -> Prop)
+| Γ, σ => ∀ x,
+  (Γ[x] ≠ ★ -> LR ξ Γ[x] ↑(σ x))
+  ∧ (Γ[x] = ★ -> Value (σ x))
+
+@[simp]
+def SemanticTyping Γ t A := ∀ ξ σ, Admissible ξ -> ΓR ξ Γ σ -> LR ξ A t[σ]
+
+local notation:170 Γ:170 " ⊨ " t:170 " : " A:170 => SemanticTyping Γ t A
+
+theorem Reducible.sn : Reducible (SN Red) := by
+  constructor
+  case _ => simp
+  case _ =>
+    intro s t h r
+    apply SN.preservation_step h r
+  case _ =>
+    intro s h1 h2
+    apply SN.sn h2
+  case _ =>
+    intro t r h
+    apply SN.monotone r h
+
+theorem Admissible.sn : Admissible (λ _ => SN Red) := by
+  intro x; apply Reducible.sn
+
+theorem Reducible.var x : Reducible P -> P #x := by
+  intro h; apply h.neu_acc; simp
+  intro t r; cases r
+
+theorem Reducible.cons : Reducible P -> Admissible ξ -> Admissible (P::ξ) := by
+  intro h1 h2 x
+  cases x <;> simp [*]
+  case _ x => apply h2 x
+
+theorem LR.monotone (r : Ren) : Admissible ξ -> LR ξ A t -> LR ξ A t[r] := by
+  intro ad h; cases A
+  case var x =>
+    simp at *
+    apply (ad x).mono r h
+  case ctor n v ts =>
+    cases v
+    case arr =>
+      simp at *; intro r' a h1
+      replace h := h (r' ∘ r) a h1
+      rw [Ren.to_compose] at h; apply h
+    all_goals simp at *; apply SN.monotone; apply h
+  case bind n v ts b =>
+    cases v
+    case all =>
+      simp at *; intro r' C a h1 h2
+      replace h := h (r' ∘ r) C a h1 h2
+      rw [Ren.to_compose] at h; apply h
+    all_goals simp at *; apply SN.monotone; apply h
+
+theorem LR.reducible A : Admissible ξ -> Reducible (LR ξ A) := by
+  intro ad
+  induction A generalizing ξ
+  case var x => simp; apply ad
+  case ctor v ts ih =>
+    cases v
+    all_goals try solve | simp; apply Reducible.sn
+    have ih1 := ih (Fin.ofNat 2 0) ad; simp at ih1
+    have ih2 := ih (Fin.ofNat 2 1) ad; simp at ih2
+    rw [<-Vec.eta2 (t := ts)]
+    constructor
+    case subset =>
+      intro t q
+      have lem := q id #0 (Reducible.var 0 ih1); simp at lem
+      replace lem := ih2.subset lem
+      apply SN.preimage (· :@ #0) t _ lem
+      simp; intro x y
+      apply Red.app1
+    case closed =>
+      intro s t q r re a la
+      have lem1 := q re a la
+      have lem2 : (s[re] :@ a) ~> (t[re] :@ a) := by
+        apply Red.ctor _ 0 <;> simp
+        apply Red.subst _ r
+      apply ih2.closed lem1 lem2
+    case neu_acc =>
+      intro s q1 q2 re a la
+      have lem := ih1.subset la
+      induction lem; case _ x lem ih3 =>
+      apply ih2.neu_acc; rfl; intro t r
+      replace r := Red.app_inv r
+      rcases r with ⟨A, b, e1, e2⟩ | ⟨f', e, r⟩ | ⟨a', e, r⟩
+      case _ =>
+        cases s <;> simp at e1
+        rcases e1 with ⟨e1, e2, e3, e4⟩
+        subst e1; simp at *; subst e2; subst e3; subst e4
+        simp at q1
+      case _ =>
+        subst e
+        have lem : ∃ z, s ~> z ∧ f' = z[re] := Red.antirename re r
+        rcases lem with ⟨z, h1, h2⟩
+        replace q2 := q2 _ h1; simp at q2
+        subst h2; apply q2 re x la
+      case _ =>
+        subst e; apply ih3 _ r
+        apply ih1.closed la r
+    case mono =>
+      intro t r h
+      apply LR.monotone r ad; apply h
+  case bind v ts A ih1 ih2 =>
+    cases v
+    all_goals try solve | simp; apply Reducible.sn
+    constructor
+    case subset =>
+      replace ih := @ih2 ((SN Red)::ξ) (Reducible.cons Reducible.sn ad)
+      intro t q
+      have lem := q id (SN Red) #0 Reducible.sn Value.var; simp at lem
+      replace lem := ih.subset lem
+      apply SN.preimage (· :@[#0]) t _ lem
+      simp; intro x y
+      apply Red.tapp1
+    case closed =>
+      intro s t q1 r re C a q2 q3
+      replace ih := @ih2 (C::ξ) (Reducible.cons q2 ad)
+      apply ih.closed
+      apply q1 re _ a q2 q3
+      have lem : s[re] ~> t[re] := by apply Red.subst _ r
+      apply Red.tapp1 lem
+    case neu_acc =>
+      intro s q1 q2 re C a q3 q4
+      replace ih := @ih2 (C::ξ) (Reducible.cons q3 ad)
+      apply ih.neu_acc; rfl
+      intro t r
+      replace r := Red.tapp_inv r
+      rcases r with ⟨b, e1, e2⟩ | ⟨f', e, r⟩ | ⟨a', e, r⟩
+      case _ =>
+        cases s <;> simp at e1
+        rcases e1 with ⟨e1, e2, e3, e4⟩
+        subst e1; simp at *; subst e2
+        simp at q1
+      case _ =>
+        subst e
+        have lem : ∃ z, s ~> z ∧ f' = z[re] := Red.antirename re r
+        rcases lem with ⟨z, h1, h2⟩
+        replace q2 := q2 _ h1; simp at q2
+        subst h2; apply q2 re _ _ q3 q4
+      case _ => exfalso; apply Value.sound q4 _ r
+    case mono =>
+      intro t r h
+      apply LR.monotone r ad; apply h
+
+theorem LR.var : Admissible ξ -> LR ξ T #x := by
+  intro h
+  have lem := LR.reducible T h
+  apply lem.neu_acc; rfl
+  intro t r; cases r
+
+theorem LR.preservation :
+  Admissible ξ ->
+  LR ξ T s ->
+  s ~>* t ->
+  LR ξ T t
+:= by
+  intro h1 h2 h3
+  have lem := LR.reducible T h1
+  induction h3; simp [*]
+  case _ r1 r2 => apply lem.closed r2 r1
+
+theorem LR.beta_expansion :
+  Admissible ξ ->
+  SN Red t ->
+  Value B ->
+  LR ξ A b[su t::+0] ->
+  LR ξ A ((:λ[B] b) :@ t)
+:= by
+  intro ad snt vb h
+  have lem := LR.reducible A ad
+  have sns := SN.subst_preimage (lem.subset h)
+  induction sns generalizing t; case _ s sns ih1 =>
+  induction snt; case _ t snt ih2 =>
+  apply lem.neu_acc; rfl; intro u r; simp at r
+  replace r := Red.app_inv r
+  rcases r with ⟨A, b, e, r⟩ | ⟨f', e, r⟩ | ⟨a', e, r⟩
+  case _ =>
+    injection e with _ _ _ e
+    subst r; subst e; apply h
+  case _ =>
+    subst e; replace r := Red.lam_inv r
+    rcases r with ⟨B', e, r⟩ | ⟨b', e, r⟩
+    case _ => exfalso; apply Value.sound vb _ r
+    case _ =>
+      subst e
+      apply ih1 _ r; apply SN.sn snt
+      replace r := Substitutive.subst (su t::+0) r
+      apply lem.closed h r
+  case _ =>
+    subst e; apply ih2 _ r
+    replace r : s[su t::+0] ~>* s[su a'::+0] := by
+      apply Red.subst_action (su t::+0) (su a'::+0)
+      intro i; cases i <;> simp
+      apply ActionRed.su r
+      apply ActionRed.re
+    apply LR.preservation ad h r
+
+theorem LR.tbeta_expansion :
+  Admissible ξ ->
+  Value t ->
+  LR ξ A b[su t::+0] ->
+  LR ξ A ((Λ b) :@[t])
+:= by
+  intro ad vt h
+  have lem := LR.reducible A ad
+  have sns := SN.subst_preimage (lem.subset h)
+  induction sns; case _ x h ih =>
+  apply lem.neu_acc; rfl; intro s r
+  replace r := Red.tapp_inv r
+  rcases r with ⟨b, e1, e2⟩ | ⟨f', e, r⟩ | ⟨a', e, r⟩
+  case _ =>
+    injection e1 with _ _ _ e1; subst e1; subst e2
+    apply h
+  case _ =>
+    subst e; replace r := Red.tlam_inv r
+    rcases r with ⟨b', e, r⟩; subst e
+    apply ih _ r
+    have r2 := Substitutive.subst (su t::+0) r
+    apply lem.closed h r2
+  case _ => exfalso; apply Value.sound vt _ r
+
+theorem valuation_equiv_lift {ξ ζ : Nat -> Cand} :
+  (∀ i t, ξ i t <-> ζ i t) ->
+  ∀ P i t, (P::ξ) i t <-> (P::ζ) i t
+:= by
+  intro h P i t
+  cases i <;> simp; rw [h]
+
+theorem LR.valuation_equiv :
+  (∀ i t, ξ i t <-> ζ i t) ->
+  (LR ξ T t <-> LR ζ T t)
+:= by
+  intro h1
+  induction T generalizing ξ ζ t
+  case var x => apply h1
+  case ctor v ts ih =>
+    cases v <;> simp
+    have ih1 := @ih (Fin.ofNat 2 0); simp at ih1
+    have ih2 := @ih (Fin.ofNat 2 1); simp at ih2
+    apply Iff.intro
+    case _ =>
+      intro h2 r a h3
+      have lem1 := (ih1 h1).2 h3
+      replace h2 := h2 r _ lem1
+      apply (ih2 h1).1 h2
+    case _ =>
+      intro h2 r a h3
+      have lem1 := (ih1 h1).1 h3
+      replace h2 := h2 r _ lem1
+      apply (ih2 h1).2 h2
+  case bind v ts s ih1 ih2 =>
+    cases v <;> simp
+    apply Iff.intro
+    case _ =>
+      intro h2 r C a h3
+      replace h2 := h2 r C a h3
+      replace ih2 := @ih2 (C::ξ) (C::ζ) (t[r] :@[a])
+      rw [<-ih2]; apply h2
+      intro i t; cases i <;> simp; rw [h1]
+    case _ =>
+      intro h2 r C a h3
+      replace h2 := h2 r C a h3
+      replace ih2 := @ih2 (C::ξ) (C::ζ) (t[r] :@[a])
+      rw [ih2]; apply h2
+      intro i t; cases i <;> simp; rw [h1]
+
+theorem LR.rename (r : Ren) : LR ξ T[r] t <-> LR (ξ ∘ r) T t := by
+  induction T generalizing ξ r t
+  case var x => simp
+  case ctor v ts ih =>
+    cases v <;> simp
+    have ih1 := @ih (Fin.ofNat 2 0); simp at ih1
+    have ih2 := @ih (Fin.ofNat 2 1); simp at ih2
+    apply Iff.intro
+    case _ =>
+      intro h1 re a h2
+      replace h2 := (ih1 r).2 h2
+      apply (ih2 r).1; apply h1 re _ h2
+    case _ =>
+      intro h1 re a h2
+      replace h2 := (ih1 r).1 h2
+      apply (ih2 r).2; apply h1 re _ h2
+  case bind v ts s ih1 ih2 =>
+    cases v <;> simp
+    apply Iff.intro
+    case _ =>
+      intro h1 re C a h2 h3
+      have lem1 := @ih2 (C::ξ) (t[re] :@[a]) r.lift
+      have lem2 : (C::ξ) ∘ r.lift = C::ξ ∘ r := by
+        funext; case _ i t =>
+        unfold Function.comp
+        cases i <;> simp [Ren.lift]
+      rw [lem2, Ren.to_lift (S := Term)] at lem1; simp at lem1
+      apply lem1.1; apply h1; apply h2; apply h3
+    case _ =>
+      intro h1 re C a h2 h3
+      have lem1 := @ih2 (C::ξ) (t[re] :@[a]) r.lift
+      have lem2 : (C::ξ) ∘ r.lift = C::ξ ∘ r := by
+        funext; case _ i t =>
+        unfold Function.comp
+        cases i <;> simp [Ren.lift]
+      rw [lem2, Ren.to_lift (S := Term)] at lem1; simp at lem1
+      apply lem1.2; apply h1; apply h2; apply h3
+
+theorem LR.weaken : LR (P::ξ) T[+1] t <-> LR ξ T t := by
+  exact LR.rename (· + 1)
+
+theorem LR.subst : LR ξ T[σ] t <-> LR (λ i => LR ξ (σ i)) T t := by
+  induction T generalizing ξ t
+  case var => simp
+  case ctor v ts ih =>
+    cases v <;> simp
+    have ih1 := @ih (Fin.ofNat 2 0); simp at ih1
+    have ih2 := @ih (Fin.ofNat 2 1); simp at ih2
+    apply Iff.intro
+    case _ =>
+      intro h1 re a h2
+      have lem1 := (@ih1 ξ σ a).2 h2
+      replace h1 := h1 re _ lem1
+      have lem2 := (@ih2 ξ σ (t[re] :@ a)).1 h1
+      apply lem2
+    case _ =>
+      intro h1 re a h2
+      have lem1 := (@ih1 ξ σ a).1 h2
+      replace h1 := h1 re _ lem1
+      have lem2 := (@ih2 ξ σ (t[re] :@ a)).2 h1
+      apply lem2
+  case bind v ts s ih1 ih2 =>
+    cases v <;> simp
+    apply Iff.intro
+    case _ =>
+      intro h1 k C a h2 h3
+      replace h1 := h1 k C a h2 h3
+      replace ih2 := @ih2 (C::ξ) σ.lift (t[k] :@[a])
+      have lem1 : σ.lift = re 0::σ ∘ +1 := by simp
+      rw [lem1] at ih2; rw [ih2] at h1
+      rw [LR.valuation_equiv]; apply h1
+      intro i t; cases i <;> simp
+      case _ i =>
+      have lem2 : ↑((σ ∘ +1) i) = (Term.from_action (σ i))[+1] := by simp
+      rw [lem2, LR.weaken]
+    case _ =>
+      intro h1 k C a h2
+      replace h1 := h1 k C a h2
+      replace ih2 := @ih2 (C::ξ) σ.lift (t[k] :@[a])
+      have lem1 : σ.lift = re 0::σ ∘ +1 := by simp
+      rw [lem1] at ih2; rw [ih2]
+      rw [LR.valuation_equiv]; apply h1
+      intro i t; cases i <;> simp
+      case _ i =>
+      have lem2 : ↑((σ ∘ +1) i) = (Term.from_action (σ i))[+1] := by simp
+      rw [lem2, LR.weaken]
+
+theorem Term.succ_not_star_implies_not_star : A[+1] ≠ ★ -> A ≠ ★ := by
+  intro h1 h2; subst h2; simp at h1
+
+theorem ΓR.rename (r : Ren) :
+  Admissible ξ ->
+  ΓR ξ Γ σ ->
+  ΓR ξ Γ (σ ∘ r.to)
+:= by
+  intro ad h1 x
+  apply And.intro
+  case _ =>
+    intro h2
+    replace h1 := (h1 x).1 h2
+    replace h1 := LR.monotone r ad h1; simp at h1
+    apply h1
+  case _ =>
+    intro h2
+    replace h1 := (h1 x).2 h2
+    replace h1 := Value.monotone r h1; simp at h1
+    apply h1
+
+theorem ΓR.kinding_subst_value :
+  Admissible ξ ->
+  ΓR ξ Γ σ ->
+  Γ ⊢ A type ->
+  Value A[σ]
+:= by
+  intro ad cr j
+  induction j generalizing ξ σ
+  case var Γ x j => simp; apply (cr x).2 j
+  case arr ih1 ih2 =>
+    simp; apply Value.ctor; simp
+    apply Value.mk2 <;> simp
+    apply ih1 ad cr
+    apply ih2 ad cr
+  case all Γ P j ih =>
+    have lem : σ.lift = re 0::σ ∘ +1 := by simp
+    replace ih := @ih (SN Red::ξ) σ.lift; rw [lem] at ih
+    have lem : ∀ {x}, ↑((σ ∘ +1) x) = (Term.from_action (σ x))[+1] := by simp
+    simp; apply Value.bind; simp
+    apply ih; apply Reducible.cons Reducible.sn ad
+    intro x; apply And.intro _ _
+    case _ =>
+      intro h; cases x <;> simp
+      case _ => apply SN.var
+      case _ x =>
+        replace h := Term.succ_not_star_implies_not_star h
+        replace cr := (cr x).1 h
+        rw [LR.weaken]
+        rw [lem]; apply LR.monotone _ ad cr
+    case _ =>
+      intro h; cases x <;> simp; apply Value.var
+      case _ x =>
+      replace h := Term.ren_eq_star h
+      replace cr := (cr x).2 h
+      rw [lem]; apply Value.monotone _ cr
+
+theorem fundamental  : Γ ⊢ t : A -> Γ ⊨ t : A := by
+  intro j; induction j <;> simp
+  case var Γ T x j1 j2 =>
+    intro ξ σ h1 h2
+    subst j1; apply (h2 x).1
+    intro h; rw [h] at j2
+    cases j2
+  case app Γ A B f a j1 j2 ih1 ih2 =>
+    intro ξ σ h1 h2; simp at *
+    replace ih1 := ih1 ξ σ h1 h2 id a[σ]; simp at ih1
+    apply ih1
+    apply ih2 ξ σ h1 h2
+  case lam Γ A B t j1 j2 ih =>
+    intro ξ σ h1 h2 r a la; simp at *
+    replace ih := ih ((SN Red)::ξ) (su a::σ ∘ r.to) (by {
+      intro x; cases x <;> simp
+      apply Reducible.sn
+      apply h1
+    }) (by {
+      intro x; cases x <;> simp
+      case _ =>
+        apply And.intro _ _
+        case _ => intro h; rw [LR.weaken]; exact la
+        case _ =>
+          intro h
+          replace h := Term.ren_eq_star h
+          rw [h] at j1; cases j1
+      case _ x =>
+        replace h2 := h2 x
+        apply And.intro _ _
+        case _ =>
+          intro h
+          replace h := Term.succ_not_star_implies_not_star h
+          rw [LR.weaken]
+          replace h2 := LR.monotone r h1 (h2.1 h); simp at h2
+          apply h2
+        case _ =>
+          intro h
+          replace h := Term.ren_eq_star h
+          replace h2 := Value.monotone r (h2.2 h); simp at h2
+          apply h2
+    }); simp at ih
+    have lem1 := LR.reducible A h1
+    replace lem1 := lem1.subset la
+    have lem2 := ΓR.kinding_subst_value h1 (ΓR.rename r h1 h2) j1
+    apply LR.beta_expansion h1 lem1 lem2; simp
+    rw [LR.weaken] at ih; apply ih
+  case tapp Γ P P' f a j1 j2 j3 ih =>
+    intro ξ σ h1 h2; subst j3; simp at ih;
+    rw [LR.subst]
+    have lem0 : Value a[σ] := ΓR.kinding_subst_value h1 h2 j2
+    have lem1 := ih ξ σ h1 h2 id (LR ξ a) a[σ] (LR.reducible a h1) lem0; simp at lem1
+    have lem2 : ∀ i t, (LR ξ a::ξ) i t <-> (fun i => LR ξ ↑((su a::+0) i)) i t := by
+      intro i t; cases i <;> simp
+    apply (LR.valuation_equiv lem2).1 lem1
+  case tlam Γ P t j ih =>
+    intro ξ σ h1 h2 r C a rc av; simp at ih
+    apply LR.tbeta_expansion
+    apply Reducible.cons rc h1
+    apply av; simp
+    apply ih (C::ξ) (su a::σ ∘ r.to)
+    intro x; apply Reducible.cons rc h1
+    intro x; cases x <;> simp
+    case _ => apply av
+    case _ x =>
+      replace h2 := h2 x
+      apply And.intro _ _
+      case _ =>
+        intro h
+        replace h := Term.succ_not_star_implies_not_star h
+        rw [LR.weaken]
+        replace h2 := LR.monotone r h1 (h2.1 h); simp at h2
+        apply h2
+      case _ =>
+        intro h
+        replace h := Term.ren_eq_star h
+        replace h2 := Value.monotone r (h2.2 h); simp at h2
+        apply h2
+
+theorem strong_normalization : Γ ⊢ t : A -> SN Red t := by
+  intro j; have lem1 := fundamental j; simp at lem1
+  replace lem1 := lem1 (λ x => SN Red) +0
+    (by intro x; apply Reducible.sn) (by {
+      intro x; apply And.intro
+      case _ =>
+        intro h; simp
+        apply LR.var
+        apply Admissible.sn
+      case _ =>
+        intro h; simp
+        apply Value.var
+  })
+  simp at lem1
+  replace lem2 := LR.reducible A Admissible.sn
+  apply lem2.subset lem1
+
+
+end Normalization.Verison1
