OneSortHomArityGen/Term.lean
@@ -1,0 +1,155 @@
+
+import OneSortHomArityGen.Vec
+import LeanSubst
+
+open LeanSubst
+
+inductive VariantSort where
+| bind | ctor
+
+inductive Variant : VariantSort -> Nat -> Type where
+| star : Variant .ctor 0
+| app : Variant .ctor 2
+| tapp : Variant .ctor 2
+| arr : Variant .ctor 2
+| lam : Variant .bind 1
+| tlam : Variant .bind 0
+| all : Variant .bind 0
+
+inductive Term where
+| var : Nat -> Term
+| bind {n} : (v : Variant .bind n) -> Vec Term n -> Term -> Term
+| ctor {n} : (v : Variant .ctor n) -> Vec Term n -> Term
+
+protected def Term.repr (t : Term) (p : Nat) : Std.Format :=
+  match t with
+  | var x => "#" ++ Nat.repr x
+  | ctor .star _ => "★"
+  | ctor .arr ts => Term.repr (ts 0) p ++ " -> " ++ Term.repr (ts 1) p
+  | ctor .app ts => Term.repr (ts 0) p ++ " " ++ Term.repr (ts 1) p
+  | ctor .tapp ts => Term.repr (ts 0) p  ++ "[" ++ Term.repr (ts 1) p ++ "]"
+  | bind .all _ t => "∀ " ++ Term.repr t p
+  | bind .lam ts t => "λ[" ++ Term.repr (ts 0) p ++ "] " ++ Term.repr t p
+  | bind .tlam _ t => "Λ " ++ Term.repr t p
+
+instance : Repr Term where
+  reprPrec := Term.repr
+
+notation "★" => Term.ctor Variant.star Vec.nil
+prefix:max "#" => Term.var
+notation:65 f:65 " :@ " a:64 => Term.ctor Variant.app (f::a::Vec.nil)
+notation:65 f:65 " :@[" a "]" => Term.ctor Variant.tapp (f::a::Vec.nil)
+notation ":λ[" A "] " t => Term.bind Variant.lam (A::Vec.nil) t
+notation:64 A:63 " -:> " B:64 => Term.ctor Variant.arr (A::B::Vec.nil)
+notation ":∀ " t => Term.bind Variant.all Vec.nil t
+notation "Λ " t => Term.bind Variant.tlam Vec.nil t
+
+@[app_unexpander Term.ctor]
+meta def unexpand_term_ctor : Lean.PrettyPrinter.Unexpander
+| `($(_) Variant.star v[]) => `(★)
+| `($(_) Variant.app v[$f, $a]) => `($f :@ $a)
+| `($(_) Variant.tapp v[$f, $a]) => `($f :@[$a])
+| `($(_) Variant.arr v[$a, $b]) => `($a -:> $b)
+| _ => throw ()
+
+@[app_unexpander Term.bind]
+meta def unexpand_term_bind : Lean.PrettyPrinter.Unexpander
+| `($(_) Variant.lam v[$a] $t) => `(:λ[ $a ] $t)
+| `($(_) Variant.tlam v[] $t) => `(Λ $t)
+| `($(_) Variant.all v[] $t) => `(:∀ $t)
+| _ => throw ()
+
+@[simp]
+instance : Inhabited Term where
+  default := ★
+
+@[coe]
+def Term.from_action : Subst.Action Term -> Term
+| .re y => #y
+| .su t => t
+
+@[simp]
+theorem Term.from_action_id {n} : from_action (+0 n) = #n := by
+  simp [from_action, Subst.id]
+
+@[simp]
+theorem Term.from_action_succ {n} : from_action (+1 n) = #(n + 1) := by
+  simp [from_action, Subst.succ]
+
+@[simp]
+theorem Term.from_acton_re {n} : from_action (re n) = #n := by simp [from_action]
+
+@[simp]
+theorem Term.from_action_su {t} : from_action (su t) = t := by simp [from_action]
+
+instance instCoe_SubstActionTerm_Term : Coe (Subst.Action Term) Term where
+  coe := Term.from_action
+
+@[simp]
+def Term.rmap (lf : Endo Ren) (r : Ren) : Term -> Term
+| var x => var (r x)
+| ctor v ts => ctor v (λ i => rmap lf r (ts i))
+| bind v ts t => bind v (λ i => rmap lf r (ts i)) (rmap lf (lf r) t)
+
+instance : RenMap Term where
+  rmap := Term.rmap
+
+@[simp]
+def Term.smap (lf : Endo (Subst Term)) (σ : Subst Term) : Term -> Term
+| var x => σ x
+| ctor v ts => ctor v (λ i => smap lf σ (ts i))
+| bind v ts t => bind v (λ i => smap lf σ (ts i)) (smap lf (lf σ) t)
+
+instance SubstMap_Term : SubstMap Term Term where
+  smap := Term.smap
+
+@[simp]
+theorem subst_var : (#x)[σ:Term] = σ x := by
+  unfold Subst.apply; simp [SubstMap.smap]
+
+@[simp]
+theorem subst_bind
+  : (Term.bind v ts t)[σ:Term] = .bind v (λ i => (ts i)[σ:_]) t[σ.lift:_]
+:= by unfold Subst.apply; simp [SubstMap.smap]
+
+@[simp]
+theorem subst_ctor : (Term.ctor v ts)[σ:Term] = .ctor v (λ i => (ts i)[σ:_]) := by
+  unfold Subst.apply; simp [SubstMap.smap]
+
+@[simp]
+theorem Term.from_action_compose {x} {σ τ : Subst Term}
+  : (from_action (σ x))[τ] = from_action ((σ ∘ τ) x)
+:= by
+  simp [Term.from_action, Subst.compose]
+  generalize zdef : σ x = z
+  cases z <;> simp [Term.from_action]
+
+theorem apply_id {t : Term} : t[+0] = t := by
+  induction t
+  all_goals (simp at * <;> try simp [*])
+
+instance : SubstMapId Term Term where
+  apply_id := apply_id
+
+theorem apply_stable (r : Ren) (σ : Subst Term)
+  : r.to = σ -> Ren.apply (T := Term) r = Subst.apply σ
+:= by solve_stable Term, r, σ
+
+instance : SubstMapStable Term Term where
+  apply_stable := apply_stable
+
+theorem apply_compose {s : Term} {σ τ : Subst Term} : s[σ][τ] = s[σ ∘ τ] := by
+  solve_compose Term, s, σ, τ
+
+instance SubstMapCompose_Term : SubstMapCompose Term Term where
+  apply_compose := apply_compose
+
+@[simp]
+theorem ren_apply_to_var : Term.from_action (Ren.to r x) = Term.var (r x) := by
+  simp [Ren.to]
+
+theorem Term.ren_eq_star {r : Ren} : t[r] = ★ -> t = ★ := by
+  intro h; induction t generalizing r <;> simp at *
+  case _ v ts ih =>
+  cases h; case _ h1 h2 =>
+  subst h1; simp at *; apply h2
