OneSortHomArityGen/Vec.lean
@@ -1,0 +1,232 @@
+
+import LeanSubst
+open LeanSubst
+
+def Fin.cases1
+  {motive : Fin 1 -> Prop}
+  (h : motive 0)
+  (v : Fin 1) : motive v
+:= by
+  induction v using Fin.induction; simp [*]
+  case _ i _ => apply Fin.elim0 i
+
+def Fin.cases2
+  {motive : Fin 2 -> Prop}
+  (h1 : motive 0) (h2 : motive 1)
+  (v : Fin 2) : motive v
+:= by
+  induction v using Fin.induction; simp [*]
+  case _ i h =>
+    induction i using Fin.induction; simp [*]
+    case _ i h => apply Fin.elim0 i
+
+def Vec (T : Type u) (n : Nat) := Fin n -> T
+
+def Vec.nil : Vec T 0 := λ x => nomatch x
+
+def Vec.cons (t : T) (xs : Vec T n) : Vec T (n + 1)
+| n => if h : n = 0 then t else xs (Fin.pred n h)
+
+infixr:55 "::" => Vec.cons
+
+def Vec.drop : Vec T (n + 1) -> Vec T n
+| v => λ i => v (Fin.succ i)
+
+def Vec.uncons :  Vec T (n + 1) -> T × Vec T n
+| v => (v 0, drop v)
+
+protected def Vec.reprPrec [Repr T] : {n : Nat} -> Vec T n -> Nat -> Std.Format
+| 0, _, _ => ""
+| 1, v, _ => repr (v 0)
+| _ + 1, v, i =>
+  let (h, t) := uncons v
+  (repr h) ++ ", " ++ (Vec.reprPrec t i)
+
+instance [Repr T] : Repr (Vec T n) where
+  reprPrec v n := "v[" ++ Vec.reprPrec v n ++ "]"
+
+syntax "v[" withoutPosition(term,*,?) "]"  : term
+
+-- Adapted from Lean Prelude
+macro_rules
+| `(v[ $elems,* ]) => do
+  let rec expandVecList (i : Nat) (result : Lean.TSyntax `term) : Lean.MacroM Lean.Syntax := do
+    match i with
+    | 0 => pure result
+    | i + 1 => expandVecList i (<- ``(Vec.cons `$(⟨elems.getElems.get!Internal i⟩) $result))
+  let size := elems.getElems.size
+  expandVecList size (<- ``(Vec.nil))
+
+-- Adapted from Lean Prelude
+@[app_unexpander Vec.nil]
+meta def unexpandVecNil : Lean.PrettyPrinter.Unexpander
+| `($(_)) => `(v[])
+
+-- Adapted from Lean Prelude
+@[app_unexpander Vec.cons]
+meta def unexpandVecCons : Lean.PrettyPrinter.Unexpander
+| `($(_) $x $tail) =>
+  match tail with
+  | `(v[])      => `(v[$x])
+  | `(v[$xs,*]) => `(v[$x, $xs,*])
+  | `(⋯)       => `(v[$x, $tail]) -- Unexpands to `[x, y, z, ⋯]` for `⋯ : List α`
+  | _          => throw ()
+| _ => throw ()
+
+theorem Vec.nil_singleton (v1 v2 : Vec T 0) : v1 = v2 := by
+  funext; case _ i =>
+  cases i; case _ i p => cases p
+
+@[simp]
+theorem Vec.uncons_cons_cancel : uncons (h::t) = (h, t) := by
+  simp [uncons, drop]; case _ n =>
+  apply And.intro _ _
+  case _ =>
+    cases n <;> simp [cons]
+  case _ =>
+    funext; case _ i =>
+    cases i; case _ i p =>
+    cases i <;> simp [cons, Fin.pred]
+
+@[simp]
+theorem Vec.head_drop_cancel : v 0 :: drop v = v := by
+  funext; case _ i =>
+  cases i; case _ i p =>
+  cases i <;> simp [cons, drop]
+
+theorem Vec.cons_iff_uncons {t : Vec T n} : v = h::t <-> uncons v = (h, t) := by
+  apply Iff.intro
+  case _ => intro e; subst e; simp
+  case _ =>
+    intro e; simp [uncons] at e
+    cases e; case _ e1 e2 =>
+    subst e1; subst e2; simp
+
+theorem Vec.cons_destruct (v : Vec T (n + 1)) : ∃ h t, v = cons h t := by
+  generalize pdef : uncons v = p
+  cases p; case _ h t =>
+  exists h; exists t
+  rw [cons_iff_uncons]; apply pdef
+
+theorem Vec.induction
+  {motive : {n : Nat} -> Vec T n -> Prop}
+  (nc : motive Vec.nil)
+  (cc : ∀ {n t} {v : Vec T n}, motive v -> motive (t::v))
+  (v : Vec T n)
+  : motive v
+:= by
+  induction n
+  case _ => rw [nil_singleton v]; exact nc
+  case _ n ih =>
+    have lem := cons_destruct v
+    rcases lem with ⟨h, t, e⟩; subst e
+    apply cc; apply ih
+
+-- theorem Vec.induction1
+--   {motive : Vec T 1 -> Prop}
+--   (h : ∀ {t : T}, motive v[t])
+
+@[simp]
+instance : GetElem (Vec α n) (Fin n) α (λ _ _ => True) where
+  getElem xs i _ := xs i
+
+@[simp]
+theorem get_cons_head {t : Vec T n} : (h::t) 0 = h := by simp [Vec.cons]
+
+@[simp]
+theorem get_cons_tail_succ {t : Vec T n} : (h::t) (Fin.succ i) = t i := by
+  simp [Vec.cons]; intro h; cases h
+
+@[simp]
+theorem get1_0 : v[a] 0 = a := by simp
+
+@[simp]
+theorem get2_0 : v[a, b] 0 = a := by simp
+
+@[simp]
+theorem get2_1 : v[a, b] 1 = b := by simp [Vec.cons]
+
+def Vec.map (f : A -> B) (v : Vec A n) : Vec B n := λ i => f (v i)
+
+@[simp]
+theorem Vec.map_nil : Vec.map f v[] = v[] := by
+  funext; case _ x => apply Fin.elim0 x
+
+@[simp]
+theorem Vec.map_cons : Vec.map f (h::t) = (f h)::Vec.map f t := by
+  funext; case _ i =>
+  cases i using Fin.cases <;> simp [Vec.map]
+
+@[simp]
+theorem Vec.eta0 (t : Vec T 0) : t = v[] := by apply Vec.nil_singleton
+
+@[simp]
+theorem Vec.eta1 (t : Vec T 1) : v[t 0] = t := by
+  funext; case _ i =>
+  cases i using Fin.cases1; simp
+
+@[simp]
+theorem Vec.eta2 (t : Vec T 2) : v[t 0, t 1] = t := by
+  funext; case _ i =>
+  cases i using Fin.cases2 <;> simp
+
+@[simp]
+theorem Vec.inv1 {a b : Vec T 1} : a = b <-> a 0 = b 0 := by
+  apply Iff.intro; intro h; subst h; rfl
+  intro h; funext; case _ i =>
+  cases i using Fin.cases1; exact h
+
+@[simp]
+theorem Vec.inv2 {a b : Vec T 2} : a = b <-> a 0 = b 0 ∧ a 1 = b 1 := by
+  apply Iff.intro; intro h; subst h; simp
+  intro h; funext; case _ i =>
+  cases i using Fin.cases2 <;> simp [*]
+
+def Vec.update (i : Fin n) (t : T) (ts : Vec T n) : Vec T n
+| x => if i = x then t else ts x
+
+@[simp]
+theorem Vec.update_eq : update i t ts i = t := by simp [update]
+
+theorem Vec.update_neq : ∀ j ≠ i, update i t ts j = ts j := by
+  simp [update]; intro j h1 h2
+  exfalso; apply h1; rw [h2]
+
+theorem Vec.update_stable i t {ts ts' : Vec T n} :
+  (∀ j ≠ i, ts j = ts' j) ->
+  ∀ j ≠ i, ts j = update i t ts' j
+:= by
+  intro h1 j h2; simp [update, *]
+  intro h3; exfalso; apply h2; rw [h3]
+
+def Vec.beq [BEq T] : {n : Nat} -> Vec T n -> Vec T n -> Bool
+| 0, _, _ => true
+| _ + 1, v1, v2 =>
+  let (h1, t1) := Vec.uncons v1
+  let (h2, t2) := Vec.uncons v2
+  h1 == h2 && Vec.beq t1 t2
+
+instance [BEq T] : BEq (Vec T n) where
+  beq := Vec.beq
+
+variable {S T : Type} [RenMap T] [SubstMap S T]
+
+@[simp]
+theorem Vec.subst_cons {t : Vec S n} {σ : Subst T}
+  : ((h::t) i)[σ:T] = (h[σ:_]::map (·[σ:_]) t) i
+:= by
+  induction i using Fin.induction <;> simp at *
+  case _ i ih =>
+    cases n; apply Fin.elim0 i
+    case _ n =>
+    cases i using Fin.cases <;> simp [Vec.map] at *
+
+-- @[simp]
+-- theorem Vec.subst_size1 {t : T} :
+--   (v[t] i)[σ] = (t[σ]::mk0) i
+-- := by sorry
+
+-- @[simp]
+-- theorem Vec.subst_size2 {t1 t2 : T} :
+--   (v[t1, t2] i)[σ] = (t1[σ]::t2[σ]::mk0) i
+-- := by sorry
