README.md
@@ -1,10 +1,13 @@
 # lean-sysf
 
 
-# Notes
+# OneSortHomArityGen
 
-strengthening of kinding is needed for substitution of typing
+This development uses single-sorted arity-generic syntax with homogenous substitutions
 
-this should be avoidable by annotating variables and context entries with their sort (term or type)
+Notable consequences:
+- There needs to be an explicit kinding relation to pick out types
+- The typing and kinding relation share the same context
+- Substitution assumptions have to be phrased relative to type or term replacements
+- Strong normalization requires a restriction on the argument of type application
 
-but non-annotated variables is "closer" to the original setup of System F
